added reachable constraint in lts safe and removed wf_frame check in small step linking semantics

common/SmallstepLinking.v
@@ -19,6 +19,32 @@ Ltac subst_dep :=
       idtac
   end.
 
+Inductive reachable {liA liB st} (L: lts liA liB st) (s: st) : Prop :=
+| initial_reach: forall q s0 t,
+    initial_state L q s0 ->
+    Star L s0 t s ->
+    reachable L s
+| external_reach: forall r s1 s2 t,
+    (* s1 also must be reachable *)
+    reachable L s1 ->
+    after_external L s1 r s2 ->
+    Star L s2 t s ->
+    reachable L s.
+
+Lemma step_reachable {liA liB st} (L: lts liA liB st) s1 t s2:
+  Step L s1 t s2 ->
+  reachable L s1 ->
+  reachable L s2.
+Proof.
+  intros STEP REA.
+  inv REA.
+  - eapply initial_reach; eauto.
+    eapply star_right; eauto.
+  - eapply external_reach; eauto.
+    eapply star_right; eauto.
+Qed.
+
+
 Section LINK.
   Context {li} (L: bool -> semantics li li).
   Let I := bool.
@@ -37,20 +63,26 @@ Section LINK.
     Inductive wf_frame : frame -> Prop :=
     | wf_frame_intro: forall i s q,
         at_external (L i se) s q ->
+        reachable (L i se) s ->
         wf_frame (st i s).
 
-    Definition wf_state st := Forall wf_frame st.
+    Inductive wf_state : state -> Prop :=
+    | wf_state_nil: wf_state nil
+    | wf_state_cons: forall i s k,
+        reachable (L i se) s ->
+        Forall wf_frame k ->
+        wf_state (st i s :: k).      
     
     Inductive step: state -> trace -> state -> Prop :=
-      | step_internal i s t s' k (WF: wf_state k):
+      | step_internal i s t s' k :
           Step (L i se) s t s' ->
           step (st i s :: k) t (st i s' :: k)
-      | step_push i j s q s' k (WF: wf_state k):
+      | step_push i j s q s' k :
           Smallstep.at_external (L i se) s q ->
           valid_query (L j se) q = true ->
           Smallstep.initial_state (L j se) q s' ->
           step (st i s :: k) E0 (st j s' :: st i s :: k)
-      | step_pop i j s sk r s' k (WF: wf_state (st j sk :: k)):
+      | step_pop i j s sk r s' k :
           Smallstep.final_state (L i se) s r ->
           Smallstep.after_external (L j se) sk r s' ->
           step (st i s :: st j sk :: k) E0 (st j s' :: k).
@@ -62,13 +94,13 @@ Section LINK.
           initial_state q (st i s :: nil).
 
     Inductive at_external: state -> query li -> Prop :=
-      | at_external_intro i s q k (WF: wf_state k):
+      | at_external_intro i s q k:
           Smallstep.at_external (L i se) s q ->
           (forall j, valid_query (L j se) q = false) ->
           at_external (st i s :: k) q.
 
     Inductive after_external: state -> reply li -> state -> Prop :=
-      | after_external_intro i s r s' k (WF: wf_state k):
+      | after_external_intro i s r s' k:
           Smallstep.after_external (L i se) s r s' ->
           after_external (st i s :: k) r (st i s' :: k).
 
@@ -101,7 +133,7 @@ Section LINK.
 
   (** * Properties *)
 
-  Lemma star_internal se i s t s' k (WF: wf_state se k):
+  Lemma star_internal se i s t s' k:
     Star (L i se) s t s' ->
     star (fun _ => step se) tt (st i s :: k) t (st i s' :: k).
   Proof.
@@ -109,13 +141,78 @@ Section LINK.
     constructor; auto.
   Qed.
 
-  Lemma plus_internal se i s t s' k (WF: wf_state se k):
+  Lemma plus_internal se i s t s' k:
     Plus (L i se) s t s' ->
     plus (fun _ => step se) tt (st i s :: k) t (st i s' :: k).
   Proof.
     destruct 1; econstructor; eauto using step_internal, star_internal.
   Qed.
 
+  (** Continuation of reachable state is well formed *)
+
+  
+  Lemma step_wf_state se s1 t s2:
+    Step (semantics se) s1 t s2 ->
+    wf_state se s1 ->
+    wf_state se s2.
+  Proof.
+    intros STEP WF.
+    inv STEP.
+    - inv WF. subst_dep.
+      econstructor; auto.
+      eapply step_reachable; eauto.
+    - econstructor; eauto.
+      eapply initial_reach; eauto.
+      econstructor; eauto.
+      inv WF. subst_dep.
+      econstructor; eauto.
+      econstructor; eauto.
+    - inv WF. subst_dep. inv H5.
+      econstructor; eauto.
+      eapply external_reach; eauto.
+      inv H4. subst_dep. auto.
+      eapply star_refl.
+  Qed.
+  
+  Lemma star_wf_state se s1 t s2:
+      Star (semantics se) s1 t s2 ->
+      wf_state se s1 ->
+      wf_state se s2.
+  Proof.
+    induction 1; auto.
+    intros WF. eapply IHstar.
+    inv H.
+    - eapply step_wf_state.
+      eapply step_internal. eauto.
+      auto.
+    - simpl. constructor.
+      econstructor; eauto.
+      eapply star_refl.
+      inv WF. subst_dep.
+      econstructor; eauto.
+      econstructor; eauto.
+    - simpl in *. inv WF. subst_dep.
+      inv H6.
+      econstructor; eauto.
+      inv H5. subst_dep.
+      eapply external_reach; eauto.
+      eapply star_refl.
+  Qed.
+  
+  Lemma reachable_wf_state: forall se (s: list frame),
+      reachable (semantics se) s ->
+      wf_state se s.
+  Proof.
+    induction 1.
+    - inv H. eapply star_wf_state; eauto.
+      constructor. eapply initial_reach; eauto. eapply star_refl.
+      constructor.
+    - eapply star_wf_state; eauto.
+      inv H0. inv IHreachable. subst_dep.
+      econstructor; eauto. eapply external_reach; eauto.
+      eapply star_refl.
+  Qed.
+        
   (** * Receptiveness and determinacy *)
 
   Lemma semantics_receptive:
@@ -180,7 +277,7 @@ Section LINK.
     - destruct 1. inversion 1; subst_dep.
       eapply sd_final_determ; eauto.
   Qed.
-  
+
 End LINK.
 
 (** * Compatibility with forward simulations *)
@@ -211,8 +308,6 @@ Section FSIM.
 
   Inductive match_contframes wk wk': frame L1 -> frame L2 -> Prop :=
     match_contframes_intro i s1 s2:
-      forall (WF: forall q1, Smallstep.at_external (L1 i se1) s1 q1 ->
-                   exists q2, Smallstep.at_external (L2 i se2) s2 q2),
       match_senv cc wk' se1 se2 ->
       (forall r1 r2 s1', match_reply cc wk r1 r2 ->
        Smallstep.after_external (L1 i se1) s1 r1 s1' ->
@@ -241,21 +336,6 @@ Section FSIM.
 
   (** ** Simulation properties *)
 
-  Lemma wf_state_simulation:
-    forall wk k1 k2, match_cont wk k1 k2 -> wf_state L1 se1 k1 -> wf_state L2 se2 k2. 
-  Proof.
-    intros until k2. intros MCONT WF.
-    induction MCONT.
-    - inv WF. econstructor.
-      + inv H. inv H2.
-        eapply inj_pair2 in H5. subst.
-        eapply WF in H4. destruct H4.
-        econstructor; eauto.
-      + exploit IHMCONT.
-        red. auto. auto.
-    - constructor.
-  Qed.
-  
   Lemma step_simulation:
     forall idx s1 s2 t s1', match_states idx s1 s2 -> step L1 se1 s1 t s1' ->
     exists idx' s2',
@@ -267,8 +347,6 @@ Section FSIM.
     destruct Hs1'; inv Hs.
     - (* internal step *)
       inv H3; subst_dep. clear idx0.
-      (* match_cont implies wf_state *)
-      exploit wf_state_simulation; eauto. intros WFK2.
       edestruct @fsim_simulation as (idx' & s2' & Hs2' & Hs'); eauto using fsim_lts.
       eexists (existT _ i idx'), _. split.
       * destruct Hs2'; [left | right]; intuition eauto using star_internal, plus_internal.
@@ -276,8 +354,6 @@ Section FSIM.
       * econstructor; eauto. econstructor; eauto.
     - (* cross-component call *)
       inv H5; subst_dep. clear idx0.
-      (* match_cont implies wf_state *)
-      exploit wf_state_simulation; eauto. intros WFK2.      
       edestruct @fsim_match_external as (wx & qx2 & Hqx2 & Hqx & Hsex & Hrx); eauto using fsim_lts.
       pose proof (fsim_lts (HL j) _ _ Hsex (Hse1 j)).
       edestruct @fsim_match_initial_states as (idx' & s2' & Hs2' & Hs'); eauto.
@@ -292,11 +368,6 @@ Section FSIM.
       inv H6. inv H8; subst_dep. edestruct H10 as (idx' & s2' & Hs2'& Hs'); eauto.
       eexists (existT _ j idx'), _. split.
       + left. apply plus_one. eapply step_pop; eauto.
-        inv WF. inv H6. eapply inj_pair2 in H12. subst.
-        econstructor.
-        exploit WF0; eauto. intros (q2 & ATEXT).
-        econstructor; eauto.
-        eapply wf_state_simulation; eauto.
       + repeat (econstructor; eauto).
   Qed.
 
@@ -332,21 +403,18 @@ Section FSIM.
     exists idx' s2', after_external L2 se2 s2 rx2 s2' /\ match_states idx' s1' s2'.
   Proof.
     clear - HL Hse1.
-    intros idx s1 s2 q1 Hs Hq1. destruct Hq1 as [i s1 qx1 k1 WF Hqx1 Hvld].
+    intros idx s1 s2 q1 Hs Hq1. destruct Hq1 as [i s1 qx1 k1 Hqx1 Hvld].
     inv Hs. inv H2. subst_dep. clear idx0.
     pose proof (fsim_lts (HL i) _ _ H1 H5) as Hi.
     edestruct @fsim_match_external as (wx & qx2 & Hqx2 & Hqx & Hsex & H); eauto.
     exists wx, qx2. intuition idtac.
-    + constructor.
-      eapply wf_state_simulation; eauto.
-      eauto.
+    + constructor. eauto.
       intros j. pose proof (fsim_lts (HL j) _ _ Hsex (Hse1 j)).
       erewrite fsim_match_valid_query; eauto.
     + inv H2; subst_dep.
       edestruct H as (idx' & s2' & Hs2' & Hs'); eauto.
       eexists (existT _ i idx'), _.
       split; repeat (econstructor; eauto).
-      eapply wf_state_simulation; eauto.
   Qed.
 
   Lemma semantics_simulation sk1 sk2:
