common/SmallstepLinkingSafe.v
@@ -8,8 +8,6 @@ Require Import Linking.
 Require Import Classical.
 Require Import Invariant.
 
-Parameter mem_error : forall liA liB st, lts liA liB st -> st -> Prop.
-
 (** Module safety : similar to the preservation of invariant in LTS *)
 
 Definition safe {liA liB st} (L: lts liA liB st) (s: st) : Prop :=
@@ -17,11 +15,11 @@ Definition safe {liA liB st} (L: lts liA liB st) (s: st) : Prop :=
   \/ (exists q, at_external L s q)
   \/ (exists t, exists s', Step L s t s').
 
-Definition partial_safe {liA liB st} (L: lts liA liB st) (s: st) : Prop :=
-  (exists r, final_state L s r)
-  \/ (exists q, at_external L s q)
-  \/ (exists t, exists s', Step L s t s')
-  \/ (mem_error liA liB st L s).
+(* Definition partial_safe {liA liB st} mem_error (L: lts liA liB st) (s: st) : Prop := *)
+(*   (exists r, final_state L s r) *)
+(*   \/ (exists q, at_external L s q) *)
+(*   \/ (exists t, exists s', Step L s t s') *)
+(*   \/ (mem_error liA liB st L s). *)
 
 
 (** TODO: generalize safe/partial_safe to module linking and show that
@@ -30,7 +28,7 @@ safe/partial_safe *)
 
 Record lts_safe {liA liB S} se (L: lts liA liB S) (IA: invariant liA) (IB: invariant liB) (SI: _ -> S -> Prop) w :=
   {
-    step_safe s t s':
+    step_safe s t s' (REACH: reachable L s):
       (* SI L s -> *)
       Step L s t s' ->
       SI L s';
@@ -41,7 +39,7 @@ Record lts_safe {liA liB S} se (L: lts liA liB S) (IA: invariant liA) (IB: invar
     initial_safe q s:
       initial_state L q s ->
       SI L s;
-    external_safe s q:
+    external_safe s q (REACH: reachable L s):
       at_external L s q ->
       exists wA, symtbl_inv IA wA se /\ query_inv IA wA q /\
               forall r, reply_inv IA wA r ->
@@ -49,7 +47,7 @@ Record lts_safe {liA liB S} se (L: lts liA liB S) (IA: invariant liA) (IB: invar
                    (exists s', after_external L s r s')
                    (* after external safe *)
                    /\ (forall s', after_external L s r s' -> SI L s');
-    final_safe s r:
+    final_safe s r (REACH: reachable L s):
       final_state L s r ->
       reply_inv IB w r;
   }.
@@ -70,7 +68,7 @@ Lemma safe_internal {li} (I: invariant li) L1 L2: forall i sk se s k w,
       (VALIDSE: forall i, Genv.valid_for (skel (L i)) se)
       (SAFE: forall i, module_safe (L i) I I safe)
       (STSAFE: safe (L i se) s)
-      (WFFRAMES: Forall (wf_frame L se) k),
+      (WFSTATE: wf_state L se (st L i s :: k)),
       safe (SmallstepLinking.semantics L sk se) (st L i s :: k).
 Proof.
   intros.
@@ -81,18 +79,17 @@ Proof.
     -- destruct f.
        right. right.
        (* s0 in in at_external state *)
-       inv WFFRAMES. inv H1. eapply inj_pair2 in H3. subst.
-       generalize (external_safe _ _ _ _ _ _ (SAFE i0 _ _ (VALIDSE i0) INV) s0 q H0).
+       inv WFSTATE. subst_dep. inv H3. inv H2. subst_dep.
+       generalize (external_safe _ _ _ _ _ _ (SAFE i0 _ _ (VALIDSE i0) INV) s0 q H5 H3).
        intros (wA & SYMBINV & QINV & AFTER).
-       generalize (final_safe _ _ _ _ _ _ (SAFE i _ _ (VALIDSE i) SYMBINV) _ _ FINAL).
+       generalize (final_safe _ _ _ _ _ _ (SAFE i _ _ (VALIDSE i) SYMBINV) _ _ H1 FINAL).
        intros WR.
        generalize (AFTER _ WR).
        intros ((s0' & AFTER1) & SAFTER).
        do 2 eexists.
        eapply step_pop; eauto.
-       constructor. econstructor.
-       eauto. eauto.             
-  * generalize (external_safe _ _ _ _ _ _ (SAFE i _ _ (VALIDSE i) INV) s q EXT).
+  * inv WFSTATE. subst_dep.
+    generalize (external_safe _ _ _ _ _ _ (SAFE i _ _ (VALIDSE i) INV) s q H1 EXT).
     intros (wA & SYMBINV & QINV & AFTER).
     destruct (valid_query (L i se) q) eqn: VQ1.
     -- right. right.
@@ -126,7 +123,7 @@ Proof.
               simpl. eauto. eauto.
               intros. destruct j; simpl; auto.
   * right. right. do 2 eexists.
-    eapply step_internal. simpl. eauto. eauto.
+    eapply step_internal. simpl. eauto.
 Qed.
   
 Lemma compose_safety {li} (I: invariant li) L1 L2 L:
@@ -148,32 +145,41 @@ Proof.
   assert (SAFE: forall i, module_safe (L i) I I safe).
   destruct i; simpl; auto.
   constructor.
-  - intros s t s' STEP.
+  - intros s t s' REACH STEP.
+    eapply reachable_wf_state in REACH.
     inv STEP.
     + (* destruct i; simpl in H. *)
       assert (A: safe (L i se) s0). right. right. eauto.
       assert (B: safe (L i se) s'0). {
-        eapply step_safe. eapply SAFE; eauto. eauto. }
+        eapply step_safe; eauto. eapply SAFE; eauto.
+        inv REACH. subst_dep. auto. }
       eapply safe_internal; eauto.
+      inv REACH. subst_dep. econstructor;eauto. eapply step_reachable; eauto.
     (* step_push *)
     + assert (A: safe (L i se) s0). right. left. eauto.
       assert (B: safe (L j se) s'0).
       eapply initial_safe. eapply SAFE; eauto. eauto.
       eapply safe_internal;eauto.
       constructor; eauto. econstructor; eauto.
+      eapply star_refl.
+      inv REACH. subst_dep. econstructor;eauto.
+      econstructor;eauto.
     (* step_pop *)
-    + inv WF. inv H3. eapply inj_pair2 in H5. subst.
+    + inv REACH. inv H5. subst_dep.
+      inv H6. subst_dep.
       assert (ATEXT: exists q, at_external (L j se) sk0 q).
       eauto.
       destruct ATEXT as (q1 & ATEXT).
-      generalize (external_safe _ _ _ _ _ _ (SAFE j _ _ (VALIDSE j) INV) sk0 q1 ATEXT).
+      generalize (external_safe _ _ _ _ _ _ (SAFE j _ _ (VALIDSE j) INV) sk0 q1 H5 ATEXT).
       intros (wA & SYMBINV & QINV & AFTER).
-      generalize (final_safe _ _ _ _ _ _ (SAFE i _ _ (VALIDSE i) SYMBINV) _ _ H).
+      generalize (final_safe _ _ _ _ _ _ (SAFE i _ _ (VALIDSE i) SYMBINV) _ _ H3 H).
       intros VR.
       generalize (AFTER r VR).
       intros ((s' & AFTER1) & C).
       assert (B: safe (L j se) s'0). eapply C. eauto.
       eapply safe_internal; eauto.
+      econstructor;eauto. eapply external_reach. eapply H5. eapply H0.
+      eapply star_refl.
   (* initial_progress *)
   - intros q VQ SQ. simpl in *.
     unfold SmallstepLinking.valid_query in VQ.
@@ -193,8 +199,11 @@ Proof.
     intros A.
     (* repeated work *)
     eapply safe_internal; eauto.
-  - intros s q EXT. inv EXT.
-    generalize (external_safe _ _ _ _ _ _ (SAFE i _ _ (VALIDSE i) INV) s0 q H).
+    econstructor. eapply initial_reach; eauto.
+    eapply star_refl. constructor.
+  - intros s q REACH EXT. inv EXT.
+    eapply reachable_wf_state in REACH. inv REACH. subst_dep.
+    generalize (external_safe _ _ _ _ _ _ (SAFE i _ _ (VALIDSE i) INV) s0 q H3 H).
     intros (wA & SYMBINV & QINV & AFTER).
     exists wA. split; auto. split; auto.
     intros r SR.
@@ -202,12 +211,15 @@ Proof.
     intros ((s' & AFTER1) & C).
     split. exists (st L i s' :: k). econstructor; eauto.
     intros s1' AFTER2. simpl in *. inv AFTER2. 
-    eapply inj_pair2 in H3. subst.
-    generalize (C s'0 H6). intros D.
+    subst_dep.
+    generalize (C s'0 H8). intros D.
     (* repeated work *)
     eapply safe_internal; eauto.
-  - intros s r FINAL. simpl in *.
+    econstructor; eauto. eapply external_reach; eauto.
+    eapply star_refl.    
+  - intros s r REACH FINAL.
     inv FINAL.
-    generalize (final_safe _ _ _ _ _ _ (SAFE i _ _ (VALIDSE i) INV) _ _ H).
+    apply reachable_wf_state in REACH. inv REACH. subst_dep.
+    generalize (final_safe _ _ _ _ _ _ (SAFE i _ _ (VALIDSE i) INV) _ _ H2 H).
     auto.
 Qed.
