rustfrontend/BorrowCheckSafe.v
@@ -12,29 +12,48 @@ Require Import RustIR BorrowCheckPolonius.
 
 Section BORROWCK.
 
-Variable p tp: program.
+Variable p: program.
+Variable w: inv_world wt_c.
 Variable se: Genv.symtbl.
-Hypothesis BORCHK: borrow_check_program p = OK tp.
 Hypothesis VALIDSE: Genv.valid_for (erase_program p) se.
+Hypothesis INV: symtbl_inv wt_c w se.
+Let L := semantics p se.
+Let ge := globalenv se p.
 
-Let L1 := semantics p se.
-Let L2 := semantics tp se.
+Variable sound_state: state -> Prop.
 
+Lemma sound_state_no_mem_error: forall s,
+    step_mem_error ge s -> sound_state s -> False .
+Admitted.
 
-Lemma sound_state_safe: forall s,
-    partial_safe L1 s ->
-    safe L2 s.
+(** Specific definition of partial safe *)
+Definition partial_safe (s: state) : Prop :=
+  safe L s \/ step_mem_error ge s.
+
+Lemma borrow_check_lts_safe:
+    borrow_check_program p = OK tt ->
+    lts_safe se (semantics p se) wt_c wt_c (fun _ => partial_safe) w ->
+    lts_safe se (semantics p se) wt_c wt_c safe w.
+Proof.
+  intros BORCHK PSAFE. inv PSAFE.  
+  constructor.
+  - simpl in *. intros s t s' STEP.
+    generalize (step_safe _ _ _ STEP). intros PSAFE.
+    destruct PSAFE as [|MEMERROR]. auto.
+    
+    
 Admitted.
 
 End BORROWCK.
 
 
-Lemma borrow_check_safe: forall p tp,
-    borrow_check_program p = OK tp ->
-    module_safe (semantics p) wt_c wt_c partial_safe ->
-    module_safe (semantics tp) wt_c wt_c safe.
-Proof.
-  intros p tp BORCHK MSAFE.
-  red. intros w se VALIDSE SYMBINV.
-Admitted.
+
+(* Lemma borrow_check_safe: forall p, *)
+(*     borrow_check_program p = OK tt -> *)
+(*     module_safe (semantics p) wt_c wt_c partial_safe -> *)
+(*     module_safe (semantics p) wt_c wt_c safe. *)
+(* Proof. *)
+(*   intros p BORCHK MSAFE. *)
+(*   red. intros w se VALIDSE SYMBINV. *)
+(* Admitted. *)
     
