Makefile
@@ -170,6 +170,7 @@ RUSTFRONTENT=Rusttypes.v Rustsyntax.v RustlightBase.v RustIR.v\
   RustIRgen.v \
   InitAnalysis.v ElaborateDrop.v\
   BorrowCheckDomain.v ReplaceOrigins.v BorrowCheckPolonius.v\
+  BorrowCheckSafe.v\
   Clightgen.v Clightgenspec.v Clightgenproof.v\
   RustOp.v
 
